src/program_proof/mvcc/txn_abort.v
@@ -1,0 +1,26 @@
+From Perennial.program_proof.mvcc Require Import txn_common txnmgr_deactivate.
+
+Section program.
+Context `{!heapGS Σ, !mvcc_ghostG Σ}.
+
+Theorem wp_txn__Abort txn γ τ :
+  {{{ own_txn txn γ τ }}}
+    Txn__Abort #txn
+  {{{ RET #(); own_txn_uninit txn γ }}}.
+Proof.
+  iIntros (Φ) "Htxn HΦ".
+  wp_call.
+
+  (***********************************************************)
+  (* txn.txnMgr.deactivate(txn.sid, txn.tid)                 *)
+  (***********************************************************)
+  iNamed "Htxn".
+  iNamed "Himpl".
+  do 3 wp_loadField.
+  wp_apply (wp_txnMgr__deactivate with "HtxnmgrRI Hactive").
+  wp_pures.
+  iApply "HΦ".
+  eauto 20 with iFrame.
+Qed.
+
+End program.
