src/program_proof/mvcc/txn_acquire.v
@@ -1,0 +1,14 @@
+From Perennial.program_proof.mvcc Require Import txn_common.
+
+Section program.
+Context `{!heapGS Σ, !mvcc_ghostG Σ}.
+
+Theorem wp_txn__acquire txn γ τ :
+  {{{ own_txn txn γ τ }}}
+    Txn__acquire #txn
+  {{{ (ok : bool), RET #ok;
+      if ok then own_txn_ready txn γ τ else own_txn txn γ τ
+  }}}.
+Admitted.
+
+End program.
