src/program_proof/mvcc/txn_commit.v
@@ -3,8 +3,14 @@ From Perennial.program_proof.mvcc Require Import txn_common.
 Section program.
 Context `{!heapGS Σ, !mvcc_ghostG Σ}.
 
+Theorem wp_txn__Commit_false txn γ τ :
+  {{{ own_txn_ready txn γ τ }}}
+    Txn__Commit #txn
+  {{{ (ok : bool), RET #ok; False }}}.
+Admitted.
+
 Theorem wp_txn__Commit txn γ τ :
-  {{{ own_txn txn γ τ }}}
+  {{{ own_txn_ready txn γ τ }}}
     Txn__Commit #txn
   {{{ (ok : bool), RET #ok; own_txn_uninit txn γ }}}.
 Admitted.
